Valaig/Aig/FromStd.lean
@@ -1,0 +1,91 @@
+import Valaig.Aig.Basic
+import Valaig.Aig.Lemmas
+import Std.Sat.AIG.Basic
+
+-- Convert from a Std.Sat.AIG to our sequential Aig
+
+namespace Valaig.Aig
+
+variable {α : Type} [DecidableEq α] [Hashable α]
+
+open Std.Sat AIG
+
+inductive RelabelledAtom (aig : AIG α) where
+| input
+  (symbol : String := "")
+  : RelabelledAtom aig
+| latch
+  (next : aig.Ref)
+  (reset : Option aig.Ref := none)
+  (symbol : String := "")
+  : RelabelledAtom aig
+
+@[unbox, grind]
+private structure FromStdState (stdAig : AIG α) where
+  aig : Aig := .empty
+  -- A map from variable indices in stdAig (Ref.gate) to Vars in aig
+  map : Array Var := #[]
+  -- A map from the variable defined by each latch to its ref in stdAig, to
+  -- allow latch finalisation once all nodes have been visited
+  latchNexts : Std.HashMap Var stdAig.Ref := .emptyWithCapacity
+
+  hmap : ∀ {x} (_ : x ∈ map), x.validIn aig := by grind
+  hlatch : ∀ {l} (_ : l ∈ aig.latches), l.var ∈ latchNexts := by grind
+
+def fromStdAIG (stdAig : AIG α) (relabel : α -> RelabelledAtom stdAig) : (aig : Aig) × (stdAig.Ref -> Lit.In aig) :=
+  have ⟨state, hstate⟩ := go
+
+  let aig := state.aig.finaliseLatches fun latch h =>
+    let ref := state.latchNexts[latch.var]'(state.hlatch h)
+    have := ref.hgate
+    let lit := state.map[ref.gate]'(by omega) |>.toLit ref.invert
+    ⟨lit, by grind⟩
+
+  -- TODO: This duplication between this and the above is slightly annoying
+  let lookup (ref : stdAig.Ref) : Lit.In aig :=
+    have := ref.hgate
+    let lit := state.map[ref.gate]'(by omega) |>.toLit ref.invert
+    ⟨lit, by grind⟩
+
+  ⟨aig, lookup⟩
+
+where
+  go (s : FromStdState stdAig := {}) : { s : FromStdState stdAig // s.map.size ≥ stdAig.decls.size } :=
+    let idx := s.map.size
+    if hidx : idx ≥ stdAig.decls.size then 
+      ⟨s, hidx⟩
+    else
+      match heq : stdAig.decls[idx] with
+      | .false => go { s with map := s.map.push .constant, hmap := by grind }
+      | .gate rhs0 rhs1 =>
+        have hdag := stdAig.hdag (i := idx) (lhs := rhs0) (rhs := rhs1) (by omega) heq
+        let rhs0 := s.map[rhs0.gate]'hdag.left |>.toLit rhs0.invert
+        let rhs1 := s.map[rhs1.gate]'hdag.right |>.toLit rhs1.invert
+        let (eq:=_) (aig, lhs) := s.aig.addGate rhs0 rhs1
+        let map := s.map.push lhs.var
+        go { s with aig, map, hmap := by grind, hlatch := by grind }
+
+      | .atom a =>
+        match relabel a with
+        | .input symbol =>
+          let (eq :=_) (aig, lhs) := s.aig.addInput symbol
+          let map := s.map.push lhs.var
+          go { s with aig, map, hmap := by grind, hlatch := by grind }
+
+        | .latch next reset symbol =>
+          let (eq:=_) (aig, lhs) := s.aig.addLatch' (reset.map Lit.ofRef) symbol
+          let map := s.map.push lhs.var
+          let latchNexts := s.latchNexts.insert lhs next
+          let hlatch := by grind [addLatch'_latches_eq_push]
+          go { aig, map, latchNexts, hmap := by grind, hlatch }
+
+  termination_by stdAig.decls.size - s.map.size
+
+@[inline]
+def fromStdEntrypoint (entry : Entrypoint α) (relabel : α -> RelabelledAtom entry.aig) :
+    (aig : Aig) × Lit × (entry.aig.Ref -> Lit.In aig) :=
+  let ⟨aig, map⟩ := fromStdAIG entry.aig relabel
+  let lit := map entry.ref
+  ⟨aig, lit, map⟩
+
+end Valaig.Aig
