Valaig/Aig/Lemmas.lean
@@ -2,7 +2,7 @@ import Valaig.Aig.Basic
 
 namespace Valaig.Aig
 
-variable {aig : Aig}
+variable {aig : Aig} {var : Var}
 
 theorem decls_unique_inputs :
     ∀ {i j} (hi : i < aig.size) (hj : j < aig.size),
@@ -39,84 +39,180 @@ theorem latches_unique :
       aig.latches[i].var = aig.latches[j].var → i = j := by
   grind
 
+@[simp, grind! .]
+theorem empty_inputs_eq_empty :
+    empty.inputs = #[] := by
+  simp [empty]
+
+@[simp, grind! .]
+theorem empty_latches_eq_empty :
+    empty.latches = #[] := by
+  simp [empty]
+
 section
 
-variable {lit : Lit} {symbol : String}
+variable {symbol : String}
 variable {rhs0 rhs1 : Lit} {h0 : rhs0.validIn aig} {h1 : rhs1.validIn aig}
 variable {next : Lit} {reset : Option Lit}
 
-theorem addInput_size_ge :
-    (aig.addInput symbol).fst.size ≥ aig.size := by
-  simp_all [addInput]
+@[grind! .]
+theorem Var.constant_validIn : Var.constant.validIn aig := by
+  simp [Var.validIn, Var.constant, aig.aig.hzero]
 
 @[grind! .]
-theorem validIn_addInput (h : lit.validIn aig) :
-    lit.validIn (aig.addInput symbol).fst := by
-  grind [addInput_size_ge, Lit.validIn]
+theorem Lit.validIn_mk_validIn (h : var.validIn aig) {invert : Bool} :
+    Lit.mk var invert |>.validIn aig := by
+  simp_all [Var.validIn]
+
+
+theorem addInput_size_ge :
+    (aig.addInput symbol).fst.size ≥ aig.size := by
+  simp [addInput]
+
+@[grind! .]
+theorem validIn_addInput (h : var.validIn aig) :
+    var.validIn (aig.addInput symbol).fst := by
+  grind [addInput_size_ge, Var.validIn]
 
 @[grind! .]
 theorem addInput_validIn :
-    (aig.addInput symbol).snd.validIn (aig.addInput symbol).fst := by
-  simp [addInput, Lit.validIn]
+    (aig.addInput symbol).snd.var.validIn (aig.addInput symbol).fst := by
+  simp [addInput, Var.validIn]
 
-theorem addInput_notInverted :
-    ¬(aig.addInput symbol).snd.inverted := by
+theorem addInput_inputs_eq_push :
+    let (aig', input) := aig.addInput symbol
+    aig'.inputs = aig.inputs.push input := by
+  simp [addInput]
+
+@[grind! .]
+theorem addInput_latches_eq :
+    (aig.addInput symbol).fst.latches = aig.latches := by
   simp [addInput]
 
 
 theorem addLatch_size_ge :
     (aig.addLatch next reset symbol).fst.size ≥ aig.size := by
-  simp_all [addLatch]
+  simp [addLatch]
 
 @[grind! .]
-theorem validIn_addLatch (h : lit.validIn aig) :
-    lit.validIn (aig.addLatch next reset symbol).fst := by
-  grind [addLatch_size_ge, Lit.validIn]
+theorem validIn_addLatch (h : var.validIn aig) :
+    var.validIn (aig.addLatch next reset symbol).fst := by
+  grind [addLatch_size_ge, Var.validIn]
 
 @[grind! .]
 theorem addLatch_validIn:
-    (aig.addLatch next reset symbol).snd.validIn (aig.addLatch next reset symbol).fst := by
-  simp [addLatch, Lit.validIn]
+    (aig.addLatch next reset symbol).snd.var.validIn (aig.addLatch next reset symbol).fst := by
+  simp [addLatch, Var.validIn]
 
-theorem addLatch_not_inverted :
-    ¬(aig.addLatch next reset symbol).snd.inverted := by
+theorem addLatch_latches_eq_push :
+    let (aig', latch) := aig.addLatch next reset symbol
+    aig'.latches = aig.latches.push latch := by
+  simp [addLatch]
+
+@[grind! .]
+theorem addLatch_inputs_eq :
+    (aig.addLatch next reset symbol).fst.inputs = aig.inputs := by
   simp [addLatch]
 
 
 theorem addLatch'_size_ge :
     (aig.addLatch' reset symbol).fst.size ≥ aig.size := by
-  simp_all [addLatch']
+  simp [addLatch']
 
 @[grind! .]
-theorem validIn_addLatch' (h : lit.validIn aig) :
-    lit.validIn (aig.addLatch' reset symbol).fst := by
-  grind [addLatch'_size_ge, Lit.validIn]
+theorem validIn_addLatch' (h : var.validIn aig) :
+    var.validIn (aig.addLatch' reset symbol).fst := by
+  grind [addLatch'_size_ge, Var.validIn]
 
 @[grind! .]
 theorem addLatch'_validIn:
-    (aig.addLatch' reset symbol).snd.validIn (aig.addLatch' reset symbol).fst := by
-  simp [addLatch', Lit.validIn]
+    (aig.addLatch' reset symbol).snd.var.validIn (aig.addLatch' reset symbol).fst := by
+  simp [addLatch', Var.validIn]
 
-theorem addLatch'_not_inverted :
-    ¬(aig.addLatch' reset symbol).snd.inverted := by
+theorem addLatch'_latches_eq_push :
+    let (aig', latch) := aig.addLatch' reset symbol
+    aig'.latches = aig.latches.push latch := by
+  simp [addLatch']
+
+@[grind! .]
+theorem addLatch'_inputs_eq :
+    (aig.addLatch' reset symbol).fst.inputs = aig.inputs := by
   simp [addLatch']
 
 
 theorem addGate_size_ge :
     (aig.addGate rhs0 rhs1 h0 h1).fst.size ≥ aig.size := by
-  simp_all [addGate]
+  simp [addGate]
 
 @[grind! .]
-theorem validIn_addGate (h : lit.validIn aig) :
-    lit.validIn (aig.addGate rhs0 rhs1 h0 h1).fst := by
-  grind [addGate_size_ge, Lit.validIn]
+theorem validIn_addGate (h : var.validIn aig) :
+    var.validIn (aig.addGate rhs0 rhs1 h0 h1).fst := by
+  grind [addGate_size_ge, Var.validIn]
 
 @[grind! .]
 theorem addGate_validIn:
     (aig.addGate rhs0 rhs1 h0 h1).snd.validIn (aig.addGate rhs0 rhs1 h0 h1).fst := by
-  simp [addGate, Lit.validIn]
+  simp [addGate, Var.validIn]
   have (r : Std.Sat.AIG.Entrypoint Aig.Atom) := r.ref.hgate
   grind
+
+@[grind! .]
+theorem addGate_inputs_eq :
+    (aig.addGate rhs0 rhs1 h0 h1).fst.inputs = aig.inputs := by
+  simp [addGate]
+
+@[grind! .]
+theorem addGate_latches_eq :
+    (aig.addGate rhs0 rhs1 h0 h1).fst.latches = aig.latches := by
+  simp [addGate]
+
+end
+
+section
+
+variable {nextState : (latch : Latch) -> latch ∈ aig.latches -> Lit.In aig}
+variable {state : FinaliseLatchesState aig}
+
+theorem finaliseLatches.updateLatches_size_const :
+    let state' := (finaliseLatches.updateLatches aig nextState (s := state))
+    state'.latches.size = state.latches.size := by
+  intro state'
+  have := state.hsize
+  have := state'.hsize
+  omega
+
+theorem finaliseLatches.updateLatches_modified_once :
+    let state' := (finaliseLatches.updateLatches aig nextState (s := state))
+    ∀ {i} (_ : i < state'.latches.size) (_ : i < state.idx),
+      state'.latches[i] = state.latches[i]'(by grind [finaliseLatches.updateLatches_size_const]) := by
+  induction h : (state.latches.size - state.idx) generalizing state with
+  | zero => grind [updateLatches]
+  | succ n' ih =>
+    simp only [updateLatches_size_const]
+    grind [updateLatches]
+
+theorem finaliseLatches.updateLatches_next_eq_some :
+    let state' := (finaliseLatches.updateLatches aig nextState (s := state))
+    ∀ {i} (_ : i < state'.latches.size) (_ : i ≥ state.idx),
+      state'.latches[i].next.isSome := by
+  induction h : (state.latches.size - state.idx) generalizing state with
+  | zero => grind [updateLatches]
+  | succ n' ih => grind [updateLatches, updateLatches_modified_once]
+
+theorem finaliseLatches_WF :
+    aig.finaliseLatches nextState |>.WF := by
+  constructor
+  · simp only [finaliseLatches]
+    grind [finaliseLatches.updateLatches_next_eq_some, List.mem_iff_getElem, Array.mem_def]
+
+theorem finaliseLatches_aig_eq :
+    (aig.finaliseLatches nextState).aig = aig.aig := by
+  simp [finaliseLatches]
+
+@[grind! .]
+theorem validIn_finaliseLatches (h : var.validIn aig) :
+    var.validIn (aig.finaliseLatches nextState) := by
+  simp_all [finaliseLatches_aig_eq, Var.validIn]
 
 end
 
